Dijkstra/Control/Monad/Dijkstra.lean
@@ -1,0 +1,236 @@
+/-
+Copyright (c) 2022 Jun Yoshida. All rights reserved.
+Released under Apache 2.0 license as described in the file LICENSE.
+-/
+
+import Dijkstra.Init
+import Dijkstra.Control.Lawful
+import Dijkstra.Control.Monad.Hom
+import Dijkstra.Control.Monad.Rel
+
+
+/-!
+
+# Dijkstra monads
+
+A ***Dijkstra monad*** is a dependent analogue of a monad which is parametrized by a specific monad, called the *underlying monad*, so that the operations `pure` and `bind` are defined along with those on the underlying monad.
+More precisely, given monad `W : Type u → Type v`, a type-family `M : (α : Type u) → W α → Type v` is a Dijkstra monad if it is equipped with the following two operations:
+
+```lean
+dpure {α : Type u} (a : α) :  M (pure a)
+dbind {α β : Type u} {wa : W α} {wf : α → W β} : M α wa → ((a : α) → M β (wf a)) → M β (wa >>= wf)
+```
+
+In addition, these operations are supposed to satisfy dependent analogues of the ordinary monad relations.
+There is, however, a problem to write down such conditions.
+For example, one would expect that the left unitality of `dbind` can be written to be of the type `dbind (dpure a) f = f a`, thouth it is not type-correct.
+Indeed, for `a : α`, `wb : W β`, and `f : α → M β wb`, we have
+
+```lean
+#check dbind (dpure a) f -- M β (pure a >>= λ _ => wb)
+#check f a               -- M β wb
+```
+
+and it turns out that the dependent parameters are not definitionally equal (even if one has `[LawfulMonad W]`).
+This is why we need `DEq` a dependent analogue of `Eq` for type families; see [Init.lean](Dijkstra/Init.lean).
+
+-/
+
+universe u v w
+
+/-- The main structures of Dijkstra monads. -/
+class DijkstraMonad (W : Type u → Type v) [Monad W] (M : (α : Type u) → W α → Type w) where
+  dpure {α : Type u} (a : α) : M α (return a)
+  dbind {α β : Type u} {wa : W α} {wf : α → W β} : M α wa → ((a : α) → M β (wf a)) → M β (wa >>= wf)
+
+export DijkstraMonad (dpure dbind)
+
+/-- The dependent monad laws for Dijkstra monads. -/
+class DijkstraMonad.Lawful (W : Type u → Type v) [Monad W] (M : (α : Type u) → W α → Type w) [DijkstraMonad W M] where
+  --- right unitality
+  dbind_dpure {α : Type u} {wa : W α} {x : M α wa} : DEq (M α) (dbind x dpure) x
+  --- left unitality
+  dpure_dbind {α β : Type u} {wf : α → W β} (a : α) (f : (a : α) → M β (wf a)) : DEq (M β) (dbind (dpure a) f) (f a)
+  --- associativity
+  dbind_assoc {α β γ : Type u} {wa : W α} {wf : α → W β} {wg : β → W γ} (x : M α wa) (f : (a : α) → M β (wf a)) (g : (b : β) → M γ (wg b)) : DEq (M γ) (dbind (dbind x f) g) (dbind x (λ a => dbind (f a) g))
+
+namespace DijkstraMonad
+
+
+/-!
+
+## Basic lemmas
+
+-/
+
+theorem dbind_congr {W : Type u → Type v} [Monad W] {M : (α : Type u) → W α → Type w} [DijkstraMonad W M] {α β : Type u} : ∀ {wa₁ wa₂ : W α} {wf₁ wf₂ : α → W β} {x₁ : M α wa₁} {x₂ : M α wa₂} {f₁ : (a : α) → M β (wf₁ a)} {f₂ : (a : α) → M β (wf₂ a)}, DEq (M α) x₁ x₂ → (∀ a, DEq (M β) (f₁ a) (f₂ a)) → DEq (M β) (dbind x₁ f₁) (dbind x₂ f₂)
+| _, _, wf₁, wf₂, _, _, f₁, f₂, DEq.refl _, hf => by
+  have : wf₁ = wf₂ := by
+    funext a
+    exact (hf a).eq_param
+  cases this
+  have : f₁ = f₂ := by
+    funext a
+    exact (hf a).eq_of_deq
+  cases this
+  exact DEq.refl _
+
+theorem dbind_congrRight {W : Type u → Type v} [Monad W] {M : (α : Type u) → W α → Type w} [DijkstraMonad W M] {α β : Type u} : ∀ {wa : W α} {wf₁ wf₂ : α → W β} {x : M α wa} {f₁ : (a : α) → M β (wf₁ a)} {f₂ : (a : α) → M β (wf₂ a)}, (∀ a, DEq (M β) (f₁ a) (f₂ a)) → DEq (M β) (dbind x f₁) (dbind x f₂) :=
+  dbind_congr (DEq.refl _) 
+
+theorem dbind_congrLeft {W : Type u → Type v} [Monad W] {M : (α : Type u) → W α → Type w} [DijkstraMonad W M] {α β : Type u} : ∀ {wa₁ wa₂ : W α} {wf : α → W β} {x₁ : M α wa₁} {x₂ : M α wa₂} {f : (a : α) → M β (wf a)}, DEq (M α) x₁ x₂ → DEq (M β) (dbind x₁ f) (dbind x₂ f) :=
+  λ h => dbind_congr h (λ _ => DEq.refl _)
+
+
+/-!
+
+## Change of underlying monads
+
+As is the case for parametrized type families, one can translate Dijkstra monads into other along monad homomorphisms on underlying monads.
+In particular, given a monad homomorphism `F : MonadHom W₁ W₂`, we define the "push-forward" `DijkstraMonad W₁ M → DijkstraMonad W₂ (Push F M)` and the "pull-back" `DijkstraMonad W₂ M → DijkstraMonad W₁ (Pull F M)`.
+
+-/
+
+section underlying
+
+universe v₁ v₂
+
+variable {W₁ : Type u → Type v₁} [Monad W₁] {W₂ : Type u → Type v₂} [Monad W₂]
+
+/-- Pushforward of Dijkstra monads along a monad homomorphism. -/
+structure Push (F : MonadHom W₁ W₂) (M : (α : Type u) → W₁ α → Type w) (α : Type u) (wa₂ : W₂ α) : Type (max v₁ w) where
+  base : W₁ α
+  body : M α base
+  underly : F.app base = wa₂
+
+namespace Push
+
+variable {F : MonadHom W₁ W₂} {M : (α : Type u) → W₁ α → Type w}
+
+protected
+theorem eq {α : Type u} {wa₂ : W₂ α} : ∀ {x y : Push F M α wa₂}, x.base = y.base → DEq (M α) x.body y.body → x = y
+| mk _ _ _, mk _ _ _, rfl, DEq.refl _ => rfl
+
+protected
+theorem deq {α : Type u} {wa₂ wa₂': W₂ α} : ∀ {x : Push F M α wa₂} {y : Push F M α wa₂'}, x.base = y.base → DEq (M α) x.body y.body → DEq (Push F M α) x y
+| mk base _ hx, mk _ _ hy, rfl, DEq.refl _ => by
+  cases (Eq.trans hy.symm hx)
+  exact DEq.refl _
+
+instance instDijkstraMonadPush [DijkstraMonad W₁ M] : DijkstraMonad W₂ (Push F M) where
+  dpure a := {
+    base := pure a
+    body := dpure a
+    underly := F.app_pure a
+  }
+  dbind x f := {
+    base := x.base >>= (λ a => (f a).base)
+    body := dbind x.body (λ a => (f a).body)
+    underly := by
+      rw [F.app_bind, x.underly]
+      apply bind_congr
+      intro a; dsimp
+      exact (f a).underly
+  }
+
+instance instDijkstraMonadLawfulPush [LawfulMonad W₁] [DijkstraMonad W₁ M] [DijkstraMonad.Lawful W₁ M] : DijkstraMonad.Lawful W₂ (Push F M) where
+  dbind_dpure := by
+    intro α wa₂ x
+    cases x with | mk x_base x_body hx =>
+    apply Push.deq <;> dsimp [dbind, dpure]
+    . rw [bind_pure]; 
+    . exact DijkstraMonad.Lawful.dbind_dpure (M:=M)
+  dpure_dbind := by
+    intro α β wb₂ a f
+    apply Push.deq <;> dsimp [dbind, dpure]
+    . rw [pure_bind]
+    . exact DijkstraMonad.Lawful.dpure_dbind (M:=M) _ _
+  dbind_assoc := by
+    intro α β γ wa₂ wf wg x f g
+    apply Push.deq <;> dsimp [dbind, dpure]
+    . rw [bind_assoc]
+    . exact DijkstraMonad.Lawful.dbind_assoc (M:=M) _ _ _
+
+end Push
+
+/-- Pullback of Dijkstra monads along a monad homomorphisms. -/
+def Pull (F : MonadHom W₁ W₂) (M : (α : Type u) → W₂ α → Type w) (α : Type u) (wa₁ : W₁ α) : Type w :=
+  M α (F.app wa₁)
+
+namespace Pull
+
+variable {F : MonadHom W₁ W₂} {M : (α : Type u) → W₂ α → Type w}
+
+instance instDijkstraMonadPull [DijkstraMonad W₂ M] : DijkstraMonad W₁ (Pull F M) where
+  dpure {α} a := (F.app_pure a).symm.rec (motive:=λ wa _ => M α wa) (dpure a)
+  dbind {_} {β} {wa} {wf} x f :=
+    (F.app_bind wa wf).symm.rec (motive:=λ wb _=> M β wb) (dbind (M:=M) (wf:=λ a => F.app (wf a)) x f)
+
+protected
+theorem deq {α : Type u} : ∀ {w₁ w₁' : W₁ α} {x : Pull F M α w₁} {y : Pull F M α w₁'}, w₁ = w₁' → DEq (M α) x y → DEq (Pull F M α) x y
+| _, _, _, _, rfl, DEq.refl _ => DEq.refl _
+
+theorem dpure_deq [DijkstraMonad W₂ M] {α : Type u} (a : α) : DEq (β:=M α) (dpure (M:=Pull F M) a) (dpure (M:=M) a) :=
+  DEq.subst_deq
+
+theorem dbind_deq [DijkstraMonad W₂ M] {α β : Type u} {wa : W₁ α} {wf : α → W₁ β} (x : Pull F M α wa) (f : (a : α) → Pull F M β (wf a)) : DEq (β:=M β) (dbind (M:=Pull F M) x f) (dbind (M:=M) x f) :=
+  DEq.subst_deq
+
+instance instDijkstraMonadLawfulPull [LawfulMonad W₁] [DijkstraMonad W₂ M] [DijkstraMonad.Lawful W₂ M] : DijkstraMonad.Lawful W₁ (Pull F M) where
+  dbind_dpure := by
+    intro α wa₁ x
+    apply Pull.deq (bind_pure _)
+    apply DEq.trans (Pull.dbind_deq x dpure) _
+    apply DEq.trans (dbind_congrRight (W:=W₂) (M:=M) Pull.dpure_deq) _
+    exact Lawful.dbind_dpure (M:=M)
+  dpure_dbind := by
+    intro α β wf a f
+    apply Pull.deq (pure_bind _ _)
+    apply DEq.trans (Pull.dbind_deq (dpure a) f) _
+    apply DEq.trans (dbind_congrLeft (W:=W₂) (M:=M) (Pull.dpure_deq a))
+    exact Lawful.dpure_dbind (M:=M) a f
+  dbind_assoc := by
+    intro α β γ wa wf wg x f g
+    apply Pull.deq (bind_assoc _ _ _)
+    apply DEq.trans (Pull.dbind_deq _ _)
+    apply DEq.trans (dbind_congrLeft (W:=W₂) (M:=M) (Pull.dbind_deq _ _))
+    apply DEq.trans (Lawful.dbind_assoc (M:=M) _ _ _)
+    apply DEq.trans _ (Pull.dbind_deq x (λ a => dbind (f a) g)).symm
+    apply dbind_congrRight
+    intro a
+    exact (Pull.dbind_deq _ _).symm
+
+end Pull
+
+end underlying
+
+
+/-!
+
+## Dijkstra monads from monadic relations
+
+Given a monadic relation `r : MonadRel m n` for monads `m : Type u → Type v` and `n : Type u → Type w`, the associated submonad of `m × n` can be seen as a Dijkstra monad.
+Although its underlying monad is a priori the product `m × n`, we define it as a Dijkstra monad over the second monad `n`.
+In fact, the latter is obtained from the former by applying `Push` along the second projection.
+It however turns out that our direct definition has more straightforward description.
+
+-/
+
+def Graph {m : Type u → Type v} [Monad m] {W : Type u → Type w} [Monad W] (r : MonadRel m W) (α : Type u) (wa : W α) : Type v :=
+  {x : m α // r.rel x wa}
+
+namespace Graph
+
+variable {m : Type u → Type v} [Monad m] {W : Type u → Type v} [Monad W] {r : MonadRel m W}
+
+protected
+theorem deq {α : Type u} {wa₁ wa₂ : W α} : ∀ (x₁ : Graph r α wa₁) (x₂ : Graph r α wa₂), wa₁ = wa₂ → x₁.val = x₂.val → DEq (Graph r α) x₁ x₂
+| Subtype.mk _ _, Subtype.mk _ _, rfl, rfl => DEq.refl _
+
+instance instDijkstraMonadGraph : DijkstraMonad W (Graph r) where
+  dpure a := Subtype.mk (pure a) (r.rel_pure a)
+  dbind x f := Subtype.mk (x.val >>= (λ a => (f a).val)) $ r.rel_bind x.property (λ a => (f a).property)
+
+end Graph
+
+end DijkstraMonad
